secure_api/box/functor_box/Box.Indexing.fst
@@ -25,11 +25,11 @@ module Curve = Spec.Curve25519
 type id_log_region = (r:MR.rid{extends r root /\ is_eternal_region r /\ is_below r root})
 
 type honesty =
-  | UNDEFINED
   | HONEST
   | DISHONEST
+  | UNDEFINED
 
-type id_log_value = honesty
+type id_log_value = bool
 let id_log_range = fun id_log_key -> id_log_value
 let id_log_inv (id_log_kt:Type0) (m:MM.map' id_log_kt id_log_range) = True
 
@@ -43,14 +43,29 @@ abstract noeq type index_module =
     id_log: (id_log_t rgn subId) ->
     index_module
 
+val get_rgn: im:index_module -> GTot id_log_region
+let get_rgn im =
+  im.rgn
 
-type id (im:index_module) = i:(im.subId*im.subId) // add refinement once total order on subids is established{fst i <= snd i}
+val get_log: im:index_module -> GTot (id_log_t im.rgn im.subId)
+let get_log im =
+  im.id_log
+
+val recall_log: im:index_module -> ST unit
+  (requires (fun h0 -> True))
+  (ensures (fun h0 _ h1 ->
+    h0 == h1
+    /\ MR.m_contains im.id_log h1
+  ))
+let recall_log im =
+  MR.m_recall im.id_log
+
+type id (im:index_module) = i:(im.subId*im.subId){fst i <> snd i} // add refinement once total order on subids is established{fst i <= snd i}
 
 noeq type meta_id (im:index_module) =
   | ID of id im
   | SUBID of im.subId
 
-// Anything below here should probably be in the "user-module"
 #set-options "--z3rlimit 300 --max_ifuel 1 --max_fuel 1"
 assume val symmetric_id_generation (im:index_module): i1:im.subId -> i2:im.subId -> Lemma
   (requires (True))
@@ -69,84 +84,202 @@ let rec registered (im:index_module) (i:meta_id im) =
   | SUBID i' -> MR.witnessed (MM.defined im.id_log i')
   | ID (i1,i2) -> registered im (SUBID i1) /\ registered im (SUBID i2)
 
+val lemma_registered: im:index_module -> i:id im -> Lemma
+  (requires registered im (ID i))
+  (ensures
+    (let i1,i2 = i in
+    registered im (SUBID (i2))
+    /\ registered im (SUBID (i1))))
+  [SMTPat (registered im (ID i))]
+let lemma_registered im i =
+  ()
+
+val lemma_registered2: im:index_module -> i:id im -> Lemma
+    (requires (let i1,i2 = i in
+    registered im (SUBID (i2))
+    /\ registered im (SUBID (i1))))
+  (ensures registered im (ID i))
+  [SMTPat (registered im (ID i))]
+let lemma_registered2 im i =
+  ()
+
+
 // Put the correct flag here, as soon as we have flags for proof steps
 val honest: (im:index_module) -> (i:meta_id im) -> Tot (t:Type0{t ==> registered im i}) (decreases (measure_id im i))
 let rec honest (im:index_module) (i:meta_id im) =
   match i with
-  | SUBID i' -> MR.witnessed (MM.contains im.id_log i' HONEST) /\ MR.witnessed (MM.defined im.id_log i')
+  | SUBID i' -> MR.witnessed (MM.contains im.id_log i' true) /\ MR.witnessed (MM.defined im.id_log i')
   | ID (i1,i2) -> honest im (SUBID i1) /\ honest im (SUBID i2)
+
+val lemma_both_ids_honest: im:index_module -> i:id im -> Lemma
+  (requires (honest im (ID i)))
+  (ensures (
+    (let i1,i2 = i in
+    honest im (SUBID i1) /\ honest im (SUBID i2))
+  ))
+  [SMTPat (honest im (ID i))]
+let lemma_both_ids_honest im i = ()
+
+val lemma_single_id_honest: im:index_module -> i1:im.subId -> Lemma
+  (requires (honest im (SUBID i1)))
+  (ensures (
+    (forall (i2:im.subId) .
+      (i1 <> i2 /\ honest im (SUBID i2)) ==> (let ID i = ID (i1,i2) in honest im (ID i)))
+  ))
+  [SMTPat (honest im (SUBID i1))]
+let lemma_single_id_honest im i1 = ()
 
 val dishonest: (im:index_module) -> (i:meta_id im) -> Tot (t:Type0{(t /\ SUBID? i) ==> registered im i}) (decreases (measure_id im i))
 let rec dishonest im i =
   match i with
-  | SUBID i' -> MR.witnessed (MM.contains im.id_log i' DISHONEST) /\ MR.witnessed (MM.defined im.id_log i')
+  | SUBID i' -> MR.witnessed (MM.contains im.id_log i' false) /\ MR.witnessed (MM.defined im.id_log i')
   | ID (i1,i2) -> dishonest im (SUBID i1) \/ dishonest im (SUBID i2)
 
-val undefined: (im:index_module) -> (i:meta_id im) -> Tot (t:Type0{(t /\ SUBID? i) ==> registered im i}) (decreases (measure_id im i))
-let rec undefined im i =
-  match i with
-  | SUBID i' -> MR.witnessed (MM.contains im.id_log i' UNDEFINED) /\ MR.witnessed (MM.defined im.id_log i')
-  | ID (i1,i2) -> (undefined im (SUBID i1) /\ honest im (SUBID i2))
-                 \/ (honest im (SUBID i1) /\ undefined im (SUBID i2))
-                 \/ (undefined im (SUBID i1) /\ undefined im (SUBID i2))
+//val undefined: (im:index_module) -> (i:meta_id im) -> Tot (t:Type0) (decreases (measure_id im i))
+//let rec undefined im i =
+//  match i with
+//  | SUBID i' -> MR.witnessed (MM.contains im.id_log i' false) /\ MR.witnessed (MM.defined im.id_log i')
+//  | ID (i1,i2) -> undefined im (SUBID i1) \/ undefined im (SUBID i2)
 
 
-type absurd_honest (im:index_module) (i:meta_id im{registered im i /\ (undefined im i \/ dishonest im i)}) = honest im i
-type absurd_dishonest (im:index_module) (i:meta_id im{registered im i /\ (undefined im i \/ honest im i)}) = dishonest im i
-type absurd_undefined (im:index_module) (i:meta_id im{registered im i /\ (honest im i \/ dishonest im i)}) = undefined im i
-assume val lemma_honest_and_others_tot: im:index_module -> i:meta_id im{registered im i /\ (undefined im i \/ dishonest im i)} -> absurd_honest im i -> Lemma (False)
-assume val lemma_dishonest_and_others_tot: im:index_module -> i:meta_id im{registered im i /\ (undefined im i \/ honest im i)} -> absurd_dishonest im i -> Lemma (False)
-assume val lemma_undefined_and_others_tot: im:index_module -> i:meta_id im{registered im i /\ (honest im i \/ dishonest im i)} -> absurd_undefined im i -> Lemma (False)
+type absurd_honest (im:index_module) (i:meta_id im{dishonest im i}) = honest im i
+type absurd_dishonest (im:index_module) (i:meta_id im{honest im i}) = dishonest im i
+//type absurd_undefined (im:index_module) (i:meta_id im{(honest im i \/ dishonest im i)}) = undefined im i
+assume val lemma_honest_and_others_tot: im:index_module -> i:meta_id im{dishonest im i} -> absurd_honest im i -> Lemma (False)
+assume val lemma_dishonest_and_others_tot: im:index_module -> i:meta_id im{honest im i} -> absurd_dishonest im i -> Lemma (False)
+//assume val lemma_undefined_and_others_tot: im:index_module -> i:meta_id im{registered im i /\ (honest im i \/ dishonest im i)} -> absurd_undefined im i -> Lemma (False)
 
 
 val lemma_dishonest_not_others: (im:index_module) -> (i:meta_id im) -> ST unit
   (requires (fun h0 ->
-    registered im i
-    /\ dishonest im i
+    dishonest im i
   ))
   (ensures (fun h0 _ h1 ->
     ~(honest im i)
-    /\ ~(undefined im i)
+    ///\ ~(undefined im i)
     /\ h0==h1
   ))
 let lemma_dishonest_not_others im i =
-  let (j:(i:meta_id im{registered im i /\ dishonest im i})) = i in
+  let (j:(i:meta_id im{dishonest im i})) = i in
   FStar.Classical.impl_intro (lemma_honest_and_others_tot im j);
-  FStar.Classical.impl_intro (lemma_undefined_and_others_tot im j);
-  assert((honest im i \/ undefined im i)==> False)
+  assert(honest im i==> False)
 
 val lemma_honest_not_others: (im:index_module) -> (i:meta_id im) -> ST unit
   (requires (fun h0 ->
-    registered im i
-    /\ honest im i
+    honest im i
   ))
   (ensures (fun h0 _ h1 ->
     ~(dishonest im i)
-    /\ ~(undefined im i)
     /\ h0==h1
   ))
 let lemma_honest_not_others im i =
   let (j:(i:meta_id im{registered im i /\ honest im i})) = i in
   FStar.Classical.impl_intro (lemma_dishonest_and_others_tot im j);
-  FStar.Classical.impl_intro (lemma_undefined_and_others_tot im j);
-  assert((dishonest im i \/ undefined im i) ==> False)
+  assert(dishonest im i ==> False)
 
-val lemma_undefined_not_others: (im:index_module) -> (i:meta_id im) -> ST unit
+val lemma_honest_or_dishonest: im:index_module -> (i:meta_id im) -> ST unit
   (requires (fun h0 ->
     registered im i
-    /\ undefined im i
   ))
   (ensures (fun h0 _ h1 ->
-    ~(dishonest im i)
-    /\ ~(honest im i)
+    (honest im i \/ dishonest im i)
     /\ h0==h1
   ))
-let lemma_undefined_not_others im i =
-  let (j:(i:meta_id im{registered im i /\ undefined im i})) = i in
-  FStar.Classical.impl_intro (lemma_dishonest_and_others_tot im j);
-  FStar.Classical.impl_intro (lemma_honest_and_others_tot im j);
-  assert((dishonest im i \/ honest im i) ==> False)
+let rec lemma_honest_or_dishonest im i =
+  MR.m_recall im.id_log;
+  match i with
+  | ID (i1,i2) -> lemma_honest_or_dishonest im (SUBID i1) ; lemma_honest_or_dishonest im (SUBID i2)
+  | SUBID i' ->
+    MR.testify (MM.defined im.id_log i');
+    match MM.lookup im.id_log i' with
+    | Some b ->
+      if b then
+  MR.testify (MM.contains im.id_log i' true)
+             else
+  MR.testify (MM.contains im.id_log i' false)
 
+val fresh: im:index_module ->
+           i:meta_id im ->
+           h:mem ->
+           (t:Type0{
+             t ==>
+               ((ID? i ==>
+                 (let ID (i1,i2) = i in
+                 MM.fresh im.id_log i1 h
+                 /\ MM.fresh im.id_log i2 h))
+               /\ (SUBID? i ==>
+                  (let SUBID i' = i in
+                  MM.fresh im.id_log i' h
+                  /\ ~(MM.contains im.id_log i' true h))))
+           })
+
+let fresh im i h =
+  match i with
+  | SUBID i' ->
+    MM.fresh im.id_log i' h
+  | ID i' ->
+    MM.fresh im.id_log (fst i') h
+    /\ MM.fresh im.id_log (snd i') h
+
+#set-options "--z3rlimit 500 --max_ifuel 2 --max_fuel 3"
+val is_registered: im:index_module -> i:meta_id im -> ST bool
+  (requires (fun h0 -> True))
+  (ensures (fun h0 b h1 ->
+    h0 == h1
+    /\ (b ==> registered im i)
+  ))
+let rec is_registered im i =
+  MR.m_recall im.id_log;
+  match i with
+  | SUBID i' ->
+    (match MM.lookup im.id_log i' with
+    | Some _ -> true
+    | None ->
+      false)
+  | ID i' ->
+    let b1 = is_registered im (SUBID (fst i')) in
+    let b2 = is_registered im (SUBID (snd i')) in
+    if b1 then
+      MR.testify (MM.defined im.id_log ((fst i')));
+    if b2 then
+       MR.testify (MM.defined im.id_log ((snd i')));
+    b1 && b2
+
+
+val is_fresh: im:index_module -> i:meta_id im -> ST bool
+  (requires (fun h0 -> True))
+  (ensures (fun h0 b h1 ->
+    h0 == h1
+    /\ (b ==> fresh im i h0)
+    /\ (SUBID? i /\ not b ==> registered im i)
+    /\ (SUBID? i /\ not b ==> ~(fresh im i h0))
+    /\ (ID? i /\ not b ==> ~(fresh im i h1))
+    /\ (SUBID? i /\ b ==>
+      (let SUBID i' = i in
+      MM.fresh im.id_log i' h1))
+    /\ (b ==>
+    ((ID? i ==>
+      (let ID (i1,i2) = i in
+      MM.fresh im.id_log i1 h1
+      /\ MM.fresh im.id_log i2 h1))
+      ))
+  ))
+let rec is_fresh im i =
+  MR.m_recall im.id_log;
+  match i with
+  | SUBID i' ->
+    (match MM.lookup im.id_log i' with
+    | Some _ -> false
+    | None ->
+      true)
+  | ID i' ->
+    let b1 = is_fresh im (SUBID (fst i')) in
+    let b2 = is_fresh im (SUBID (snd i')) in
+    b1 && b2
+
+
+
+private val merge_honesty_states: h1:honesty -> h2:honesty -> honesty
 let merge_honesty_states h1 h2 =
   match h1,h2 with
   | HONEST,HONEST -> HONEST
@@ -154,40 +287,181 @@ let merge_honesty_states h1 h2 =
   | DISHONEST,_ -> DISHONEST
   | _,_ -> UNDEFINED
 
-#set-options "--z3rlimit 500 --max_ifuel 2 --max_fuel 2"
-val get_honesty: im:index_module -> i:meta_id im{registered im i} -> ST(h:honesty{(HONEST? h <==> (honest im i)) /\ (DISHONEST? h <==> dishonest im i) /\ (UNDEFINED? h <==> undefined im i)}) (decreases (measure_id im i))
-  (requires (fun h0 -> True))
-  (ensures (fun h0 b h1 ->
+
+#set-options "--z3rlimit 900 --max_ifuel 2 --max_fuel 1"
+val get_honesty: im:index_module -> i:meta_id im -> ST(h:honesty) (decreases (measure_id im i))
+  (requires (fun h0 ->
+    True
+  ))
+  (ensures (fun h0 h h1 ->
     modifies_none h0 h1
     /\ h0==h1
+    /\ (HONEST? h ==> (honest im i))
+    /\ (DISHONEST? h ==> dishonest im i)
+    ///\ (SUBID? i /\ (let SUBID i' = i in MM.contains im.id_log i' true h0) ==> HONEST? h )
+    ///\ (SUBID? i /\ (let SUBID i' = i in MM.contains im.id_log i' true h0) ==> honest im i )
+    ///\ (ID? i /\ (let ID (i1,i2) = i in MM.contains im.id_log i1 true h0 /\ MM.contains im.id_log i2 true h0) ==> HONEST? h )
   ))
 let rec get_honesty im i =
   MR.m_recall im.id_log;
   match i with
   | SUBID i' ->
-    (MR.testify (MM.defined im.id_log i');
-    match MM.lookup im.id_log i' with
-    |Some h ->
-      (match h with
-      | HONEST ->
-        lemma_honest_not_others im i;
-        h
-      | DISHONEST ->
-        lemma_dishonest_not_others im i;
-        h
-      | UNDEFINED ->
-        lemma_undefined_not_others im i;
-        h))
-  | ID (i1,i2) ->
-    let h1 = get_honesty im (SUBID i1) in
-    let h2 = get_honesty im (SUBID i2) in
+    if is_registered im (SUBID i') then
+      MR.testify (MM.defined im.id_log i');
+    (match MM.lookup im.id_log i' with
+    | Some b ->
+      lemma_honest_or_dishonest im (SUBID i');
+      (match b with
+      | true ->
+        lemma_honest_not_others im (SUBID i');
+        MR.testify(MM.contains im.id_log i' true);
+        HONEST
+      | false ->
+        lemma_dishonest_not_others im (SUBID i');
+        MR.testify(MM.contains im.id_log i' false);
+        DISHONEST)
+    | None ->
+      let h=get() in
+      assert(MM.fresh im.id_log i' h);
+      UNDEFINED)
+  | ID i' ->
+    let h1 = get_honesty im (SUBID (fst i')) in
+    let h2 = get_honesty im (SUBID (snd i')) in
     match merge_honesty_states h1 h2 with
     | HONEST ->
-      lemma_honest_not_others im i;
+      lemma_honest_not_others im (ID i');
       HONEST
     | DISHONEST ->
-      lemma_dishonest_not_others im i;
+      lemma_dishonest_not_others im (ID i');
       DISHONEST
     | UNDEFINED ->
-      lemma_undefined_not_others im i;
       UNDEFINED
+
+
+#set-options "--z3rlimit 900 --max_ifuel 1 --max_fuel 2"
+val get_reg_honesty: im:index_module -> i:meta_id im -> ST(h:honesty) (decreases (measure_id im i))
+  (requires (fun h0 ->
+    registered im i
+  ))
+  (ensures (fun h0 h h1 ->
+    modifies_none h0 h1
+    /\ h0==h1
+    /\ (HONEST? h <==> (honest im i))
+    /\ (DISHONEST? h <==> dishonest im i)
+    /\ (HONEST? h \/ DISHONEST? h)
+  ))
+let rec get_reg_honesty im i =
+  MR.m_recall im.id_log;
+  match i with
+  | SUBID i' ->
+    MR.testify (MM.defined im.id_log i');
+    (match MM.lookup im.id_log i' with
+    | Some b ->
+      (match b with
+      | true ->
+        lemma_honest_not_others im (SUBID i');
+        HONEST
+      | false ->
+        lemma_dishonest_not_others im (SUBID i');
+        DISHONEST))
+  | ID i' ->
+    let h1 = get_reg_honesty im (SUBID (fst i')) in
+    let h2 = get_reg_honesty im (SUBID (snd i')) in
+    match merge_honesty_states h1 h2 with
+    | HONEST ->
+      lemma_honest_not_others im (ID i');
+      HONEST
+    | DISHONEST ->
+      lemma_dishonest_not_others im (ID i');
+      DISHONEST
+
+
+// Maybe unify make_honest/dishonest to parameterized "set_honesty"
+private val make_rec_honest: im:index_module -> i:im.subId -> ST unit
+  (requires (fun h0 -> True))
+  (ensures (fun h0 _ h1 ->
+    (fresh im (SUBID i) h0 ==>
+              (MR.m_sel h1 im.id_log == MM.upd (MR.m_sel h0 im.id_log) i true
+              /\ modifies_just (Set.singleton im.rgn) h0.h h1.h
+              /\ honest im (SUBID i)))
+    /\ (~(fresh im (SUBID i) h0) ==> h0 == h1))
+  )
+let make_rec_honest im i =
+  (match MM.lookup im.id_log i with
+  | Some b -> ()
+  | None ->
+    MM.extend im.id_log i true)
+
+val make_honest: im:index_module -> i:meta_id im -> ST unit
+  (requires (fun h0 ->
+    honest im i \/ fresh im i h0
+  ))
+  (ensures (fun h0 _ h1 ->
+    honest im i
+    /\ (SUBID? i /\ fresh im i h0 ==>
+              (let SUBID i' = i in
+              MR.m_sel h1 im.id_log == MM.upd (MR.m_sel h0 im.id_log) i' true
+              /\ modifies (Set.singleton im.rgn) h0 h1))
+    /\ (SUBID? i /\ ~(fresh im i h0) ==> h0 == h1)
+    /\ (ID? i ==>
+           (let ID (i1,i2) = i in
+             ((~(fresh im (SUBID i1) h0) /\ ~(fresh im (SUBID i2) h0)) ==> h0 == h1)
+             /\ (fresh im (SUBID i1) h0 /\ ~(fresh im (SUBID i2) h0) ==> MR.m_sel h1 im.id_log == MM.upd (MR.m_sel h0 im.id_log) i1 true /\ modifies (Set.singleton im.rgn) h0 h1)
+             /\ (fresh im (SUBID i2) h0 /\ ~(fresh im (SUBID i1) h0) ==> MR.m_sel h1 im.id_log == MM.upd (MR.m_sel h0 im.id_log) i2 true /\ modifies (Set.singleton im.rgn) h0 h1)
+             /\ (fresh im (SUBID i1) h0 /\ fresh im (SUBID i2) h0 ==> MR.m_sel h1 im.id_log == MM.upd (MM.upd (MR.m_sel h0 im.id_log) i1 true) i2 true /\ modifies (Set.singleton im.rgn) h0 h1)))
+  ))
+let rec make_honest im i =
+  match i with
+    | SUBID i' ->
+      (match MM.lookup im.id_log i' with
+      | Some b -> ()
+      | None ->
+        MM.extend im.id_log i' true)
+    | ID (i1,i2) ->
+    make_rec_honest im i1;
+    make_rec_honest im i2
+
+private val make_rec_dishonest: im:index_module -> i:im.subId -> ST unit
+  (requires (fun h0 -> True))
+  (ensures (fun h0 _ h1 ->
+    (fresh im (SUBID i) h0 ==>
+              (MR.m_sel h1 im.id_log == MM.upd (MR.m_sel h0 im.id_log) i false
+              /\ modifies_just (Set.singleton im.rgn) h0.h h1.h
+              /\ dishonest im (SUBID i)))
+    /\ (~(fresh im (SUBID i) h0) ==> h0 == h1))
+  )
+let make_rec_dishonest im i =
+  (match MM.lookup im.id_log i with
+  | Some b -> ()
+  | None ->
+    MM.extend im.id_log i false)
+
+val make_dishonest: im:index_module -> i:meta_id im -> ST unit
+  (requires (fun h0 ->
+    dishonest im i \/ fresh im i h0
+  ))
+  (ensures (fun h0 _ h1 ->
+    dishonest im i
+    /\ (SUBID? i /\ fresh im i h0 ==>
+             (let SUBID i' = i in
+             MR.m_sel h1 im.id_log == MM.upd (MR.m_sel h0 im.id_log) i' false
+             /\ modifies (Set.singleton im.rgn) h0 h1))
+  /\ (SUBID? i /\ ~(fresh im i h0) ==> h0 == h1)
+  /\ (ID? i ==>
+         (let ID (i1,i2) = i in
+           ((~(fresh im (SUBID i1) h0) /\ ~(fresh im (SUBID i2) h0)) ==> h0 == h1)
+           /\ (fresh im (SUBID i1) h0 /\ ~(fresh im (SUBID i2) h0) ==> MR.m_sel h1 im.id_log == MM.upd (MR.m_sel h0 im.id_log) i1 false /\ modifies (Set.singleton im.rgn) h0 h1)
+           /\ (fresh im (SUBID i2) h0 /\ ~(fresh im (SUBID i1) h0) ==> MR.m_sel h1 im.id_log == MM.upd (MR.m_sel h0 im.id_log) i2 false /\ modifies (Set.singleton im.rgn) h0 h1)
+           /\ (fresh im (SUBID i1) h0 /\ fresh im (SUBID i2) h0 ==> MR.m_sel h1 im.id_log == MM.upd (MM.upd (MR.m_sel h0 im.id_log) i1 false) i2 false /\ modifies (Set.singleton im.rgn) h0 h1)))
+  ))
+
+let rec make_dishonest im i =
+  match i with
+  | SUBID i' ->
+    (match MM.lookup im.id_log i' with
+    | Some b -> ()
+    | None ->
+      MM.extend im.id_log i' false)
+  | ID (i1,i2) ->
+    make_rec_dishonest im i1;
+    make_rec_dishonest im i2
